\problem{Let $g:\mathbb{N}\to\mathbb{N}\in\PRF,
f:\mathbb{N}^2\to\mathbb{N}$ satisfies that
$f(x,0) = g(x)$, $f(x, y + 1) = f(f(\ldots f(f(x, y), y - 1), \ldots),0)$.
Prove that $f\in\PRF$.}

\begin{pf} \rm
 Let $G(x, 0) = x$ and $G(x, y + 1) = g(G(x, y))$,
 $F(0) = 1, F(x + 1) = F(x) + \sum_{i = 0}^{x} F(x)$. it is obvious that
 $G\in\PRF$, and $F(x) = Fib(2x) \in \PRF$.
 
 We now prove that $f(x, y) = G(x, F(y))$.
 The basis is $f(x, 0) = G(x, 1) = g(x)$, and we assume that
 $f(x, y^*) = G(x, F(y^*))$ For all $y^* \leq y$. Therefore, 

\[
 \begin{array}{rcl}
 f(x, y + 1)  & = &  \underbrace{g(g(\ldots g(}_{\sum_{i = 0}^{y} F(i)\textrm{ times}}
   f(x, y) )\ldots )) \\
 & = & \underbrace{g(g(\ldots g(}_{F(y) + \sum_{i = 0}^{y} F(i)\textrm{ times}}
   x )\ldots )) \\
   & = & G(x, F(y + 1)),
  \end{array}
\]

\noindent which means $f(x, y) = G(x, F(y))\in \PRF$. \qed
\end{pf}



